qa/lean/Ragu/Instances/Element/Invert.lean
@@ -38,6 +38,9 @@ def formal_instance : Core.Statements.GeneralFormalInstance where
       Circuits.Element.Invert.circuit,
       Circuits.Element.Invert.elaborated,
       Circuits.Element.Invert.main,
+      Circuits.Element.InvertWith.circuit,
+      Circuits.Element.InvertWith.elaborated,
+      Circuits.Element.InvertWith.main,
       Circuits.Core.AllocMul.circuit,
       Circuits.Core.AllocMul.elaborated,
       Circuits.Core.AllocMul.main]
@@ -51,6 +54,9 @@ def formal_instance : Core.Statements.GeneralFormalInstance where
       Circuits.Element.Invert.circuit,
       Circuits.Element.Invert.elaborated,
       Circuits.Element.Invert.main,
+      Circuits.Element.InvertWith.circuit,
+      Circuits.Element.InvertWith.elaborated,
+      Circuits.Element.InvertWith.main,
       Circuits.Core.AllocMul.circuit,
       Circuits.Core.AllocMul.elaborated,
       Circuits.Core.AllocMul.main]
